NoTypeFVar.v
@@ -1,0 +1,66 @@
+Require Import Termination.Tactics.
+Require Import Termination.Sets.
+Require Import Termination.Syntax.
+Require Import Termination.ErasedTermLemmas.
+Require Import Termination.ListUtils.
+Require Import Termination.FVLemmas.
+
+Definition no_type_fvar T vars :=
+  forall X, X ∈ pfv T type_var -> X ∈ vars -> False.
+
+Lemma is_erased_term_no_type_fvar:
+  forall t vars,
+    is_erased_term t ->
+    no_type_fvar t vars.
+Proof.
+  unfold no_type_fvar; repeat step || rewrite is_erased_term_tfv in *.
+Qed.
+
+Lemma no_type_fvar_open:
+  forall T vars rep k,
+    is_erased_term rep ->
+    no_type_fvar T vars ->
+    no_type_fvar (open k T rep) vars.
+Proof.
+  unfold no_type_fvar;
+    repeat step || t_fv_open || t_listutils ||
+           rewrite is_erased_term_tfv in * by steps; eauto.
+Qed.
+
+Lemma no_type_fvar_tail:
+  forall T x xs,
+    no_type_fvar T (x :: xs) ->
+    no_type_fvar T xs.
+Proof.
+  unfold no_type_fvar; repeat step; eauto.
+Qed.
+
+Lemma no_type_fvar_head:
+  forall T x xs,
+    no_type_fvar T (x :: xs) ->
+    x ∈ pfv T type_var ->
+    False.
+Proof.
+  unfold no_type_fvar; repeat step; eauto.
+Qed.
+
+Hint Immediate no_type_fvar_head: b_no_type_fvar.
+Hint Resolve no_type_fvar_tail: b_no_type_fvar.
+
+Lemma no_type_fvar_in_topen:
+  forall T vars k X,
+    no_type_fvar T vars ->
+    ~(X ∈ vars) ->
+    no_type_fvar (topen k T (fvar X type_var)) vars.
+Proof.
+  unfold no_type_fvar; repeat step || t_fv_open || t_listutils; eauto.
+Qed.
+
+Lemma no_type_fvar_append:
+  forall T vars1 vars2,
+    no_type_fvar T vars1 ->
+    no_type_fvar T vars2 ->
+    no_type_fvar T (vars1 ++ vars2).
+Proof.
+  unfold no_type_fvar; repeat step || t_listutils; eauto.
+Qed.
