ReducibilityUnused.v
@@ -17,6 +17,7 @@ Require Import Termination.TypeErasureLemmas.
 Require Import Termination.Freshness.
 Require Import Termination.EquivalentWithRelation.
 Require Import Termination.IdRelation.
+Require Import Termination.NoTypeFVar.
 
 Require Import Termination.FVLemmas.
 Require Import Termination.FVLemmasLists.
@@ -70,3 +71,84 @@ Proof.
            apply SatCons || apply reducible_unused2 ||
            (rewrite fv_subst_different_tag in * by (steps; eauto with bfv)).
 Qed.
+
+Lemma reducible_unused_middle:
+  forall X RC theta1 theta2 v T,
+    valid_interpretation theta1 ->
+    valid_interpretation theta2 ->
+    reducibility_candidate RC ->
+    no_type_fvar T (support theta1) -> (
+      reducible_values ((X,RC) :: theta1 ++ theta2) v T <->
+      reducible_values ((X,RC) :: theta2) v T
+    ).
+Proof.
+  repeat step.
+  - apply reducible_rename with T ((X, RC) :: theta1 ++ theta2) (idrel (pfv T type_var));
+      repeat step || apply valid_interpretation_append || (rewrite swap_idrel in * by steps) ||
+             t_idrel_lookup2 || t_lookupor || t_lookup_rewrite || t_lookup ||
+             unfold equivalent_with_relation, equivalent_rc_at || unfold no_type_fvar in * ||
+             unshelve eauto with falsity || exact True;
+      eauto using equal_with_idrel;
+      eauto using equivalent_rc_refl;
+    unfold equivalent_with_relation.
+
+    exists rc2; repeat step || rewrite lookupRight || apply lookupNoneSupport; eauto using equivalent_rc_refl.
+  - apply reducible_rename with T ((X, RC) :: theta2) (idrel (pfv T type_var));
+      repeat step || apply valid_interpretation_append || (rewrite swap_idrel in * by steps) ||
+             t_idrel_lookup2 || t_lookupor || t_lookup_rewrite || t_lookup ||
+             unfold equivalent_with_relation, equivalent_rc_at || unfold no_type_fvar in * ||
+             unshelve eauto with falsity || exact True;
+      eauto using equal_with_idrel;
+      eauto using equivalent_rc_refl;
+    unfold equivalent_with_relation.
+
+    exists rc1; repeat step || rewrite lookupRight || apply lookupNoneSupport; eauto using equivalent_rc_refl.
+Qed.
+
+Lemma reducible_unused_many1:
+  forall theta' theta T v,
+    no_type_fvar T (support theta') ->
+    valid_interpretation theta ->
+    valid_interpretation theta' ->
+    reducible_values (theta' ++ theta) v T ->
+    reducible_values theta v T.
+Proof.
+  induction theta';
+    repeat step || (poseNew (Mark 0 "once"); eapply IHtheta') || t_reducible_unused3 ||
+           apply valid_interpretation_append || apply valid_interpretation_all || unfold sat in * ||
+           unfold reducibility_candidate in * || instantiate_any;
+    eauto with b_no_type_fvar.
+Qed.
+
+Lemma reducible_unused_many2:
+  forall theta' theta T v,
+    no_type_fvar T (support theta') ->
+    valid_interpretation theta ->
+    valid_interpretation theta' ->
+    reducible_values theta v T ->
+    reducible_values (theta' ++ theta) v T.
+Proof.
+  induction theta';
+    repeat step || (poseNew (Mark 0 "once"); eapply IHtheta') || apply reducible_unused2 ||
+           apply valid_interpretation_append || apply valid_interpretation_all || unfold sat in * ||
+           unfold reducibility_candidate in * || instantiate_any;
+    eauto with b_no_type_fvar.
+Qed.
+
+Lemma reducible_unused_many:
+  forall theta' theta T v,
+    no_type_fvar T (support theta') ->
+    valid_interpretation theta ->
+    valid_interpretation theta' -> (
+      reducible_values (theta' ++ theta) v T <->
+      reducible_values theta v T
+    ).
+Proof.
+  intuition auto; eauto using reducible_unused_many1, reducible_unused_many2.
+Qed.
+
+Ltac t_reducible_unused3 :=
+  match goal with
+  | H: reducible_values ((?X,?RC) :: ?theta) ?v ?T |- reducible_values ?theta' ?v ?T =>
+    unify theta theta'; apply reducible_unused3 with X RC
+  end.
