StrictPositivityPull.v
@@ -1,0 +1,82 @@
+Require Import Equations.Equations.
+Require Import Equations.Subterm.
+
+Require Import Omega.
+
+Require Import Coq.Strings.String.
+Require Import Coq.Lists.List.
+
+Require Import Termination.StarInversions.
+Require Import Termination.StarRelation.
+Require Import Termination.SmallStep.
+Require Import Termination.Syntax.
+Require Import Termination.Trees.
+Require Import Termination.Tactics.
+Require Import Termination.Equivalence.
+Require Import Termination.OpenTOpen.
+
+Require Import Termination.SizeLemmas.
+
+Require Import Termination.WFLemmas.
+Require Import Termination.TWFLemmas.
+Require Import Termination.ErasedTermLemmas.
+
+Require Import Termination.ReducibilityCandidate.
+Require Import Termination.ReducibilityDefinition.
+Require Import Termination.ReducibilityLemmas.
+Require Import Termination.RedTactics.
+Require Import Termination.ReducibilityMeasure.
+Require Import Termination.ReducibilitySubst.
+Require Import Termination.ReducibilityRenaming.
+Require Import Termination.ReducibilityUnused.
+Require Import Termination.RedTactics2.
+
+Require Import Termination.IdRelation.
+Require Import Termination.EqualWithRelation.
+
+Require Import Termination.EquivalentWithRelation.
+Require Import Termination.AssocList.
+Require Import Termination.Sets.
+Require Import Termination.Freshness.
+Require Import Termination.SwapHoles.
+Require Import Termination.ListUtils.
+Require Import Termination.TOpenTClose.
+Require Import Termination.StrictPositivity.
+Require Import Termination.StrictPositivityPush.
+
+Require Import Termination.FVLemmas.
+
+Opaque makeFresh.
+Opaque Nat.eq_dec.
+Opaque reducible_values.
+Opaque strictly_positive.
+
+Ltac apply_induction_pull H :=
+  match goal with
+  | H1: non_empty ?theta ?A,
+    H2: forall_implicate _ ?ptheta ?theta' |- reducible_values (?theta' ++ _) _ ?T =>
+      apply H with (size T, index T) ptheta A
+  end.
+
+(*
+Lemma strictly_positive_push_forall:
+  forall measure T pre_theta theta theta' A v,
+    (size T, index T) = measure ->
+    wf T 0 ->
+    twf T 0 ->
+    wf A 0 ->
+    twf A 0 ->
+    valid_interpretation theta ->
+    valid_interpretation theta' ->
+    non_empty theta A ->
+    valid_pre_interpretation (fun a => reducible_values theta a A) pre_theta ->
+    strictly_positive T (support theta') ->
+    is_erased_type A ->
+    is_erased_type T ->
+    (forall a,
+      reducible_values theta a A ->
+      reducible_values (push_one a pre_theta ++ theta) v T) ->
+    forall_implicate (fun a => reducible_values theta a A) pre_theta theta' ->
+    reducible_values (theta' ++ theta) v T.
+Proof.
+*)
